```Scheme
(define (a-plus-abs-b a b)
  ((if (> b 0) + -) a b))
```
If $b > 0$, then $b = +b'$, where $b'$ is the absolute value of $b$.
If $b \leq 0$, then $b = -b'$, where $b'$ is the absolute value of $b$.

In the first case, we return `(+ a b)` =>`(+ a b')` => `(+ a (abs b))`.
In the second case, we return `(- a b)` =>`(- a (- b'))` => `(- a (- (abs b)))` => `(+ a (abs b))`.

Therefore, this procedure calculates the sum of $a$ and $|b|$. The appropriate operator ($+$ or $-$) is chosen depending on the sign of $b$.